examples/steel/arraystructs/LineStruct.fsti
@@ -1,8 +1,8 @@
 module LineStruct
 
-open Aggregates
 open AggregateRef
 open FStar.PCM
+open FStar.PCM.Extras
 open Steel.Effect
 open PointStruct
 
@@ -31,7 +31,7 @@ val _p2 : pcm_lens line_pcm point_pcm
 /// Taking pointers to the p1 and p2 fields of a line
 
 val addr_of_p1 (#p1 #p2: Ghost.erased point) (p: ref 'a line_pcm)
-: SteelT (q:ref 'a point_pcm{q == ref_focus p point_pcm _p1})
+: SteelT (q:ref 'a point_pcm{q == ref_focus p _p1})
     (p `pts_to` mk_line p1 p2)
     (fun q ->
        (p `pts_to` mk_line (one point_pcm) p2) `star`
@@ -39,13 +39,13 @@ val addr_of_p1 (#p1 #p2: Ghost.erased point) (p: ref 'a line_pcm)
 
 val un_addr_of_p1 (#p1 #p2: Ghost.erased point)
   (p: ref 'a line_pcm)
-  (q: ref 'a point_pcm{q == ref_focus p point_pcm _p1})
+  (q: ref 'a point_pcm{q == ref_focus p _p1})
 : SteelT unit
     ((p `pts_to` mk_line (one point_pcm) p2) `star` (q `pts_to` p1))
     (fun q -> p `pts_to` mk_line p1 p2)
 
 val addr_of_p2 (#p1 #p2: Ghost.erased point) (p: ref 'a line_pcm)
-: SteelT (q:ref 'a point_pcm{q == ref_focus p point_pcm _p2})
+: SteelT (q:ref 'a point_pcm{q == ref_focus p _p2})
     (p `pts_to` mk_line p1 p2)
     (fun q ->
        (p `pts_to` mk_line p1 (one point_pcm)) `star`
@@ -53,7 +53,7 @@ val addr_of_p2 (#p1 #p2: Ghost.erased point) (p: ref 'a line_pcm)
 
 val un_addr_of_p2 (#p1 #p2: Ghost.erased point)
   (p: ref 'a line_pcm)
-  (q: ref 'a point_pcm{q == ref_focus p point_pcm _p2})
+  (q: ref 'a point_pcm{q == ref_focus p _p2})
 : SteelT unit
     ((p `pts_to` mk_line p1 (one point_pcm)) `star` (q `pts_to` p2))
     (fun q -> p `pts_to` mk_line p1 p2)
